src/Iris/Proofmode/Environments.lean
@@ -24,6 +24,32 @@ def envs_entails [BI PROP] (Δ : Envs PROP) (Q : PROP) : Prop :=
   of_envs Δ.intuitionistic Δ.spatial ⊢ Q
 
 
+inductive EnvsIndex (lₚ lₛ : Nat)
+  | p : Fin lₚ → EnvsIndex lₚ lₛ
+  | s : Fin lₛ → EnvsIndex lₚ lₛ
+
+
+class AffineEnv [BI PROP] (Γ : List PROP) where
+  affine_env : ∀ p, p ∈ Γ → Affine p
+
+instance affine_env_nil [BI PROP] :
+  AffineEnv (PROP := PROP) []
+where
+  affine_env := sorry
+
+instance affine_env_cons [BI PROP] (P : PROP) (Γ : List PROP) :
+  [Affine P] →
+  [AffineEnv Γ] →
+  AffineEnv (P :: Γ)
+where
+  affine_env := sorry
+
+instance (priority := default + 10) affine_env_bi [BIAffine PROP] (Γ : List PROP) :
+  AffineEnv Γ
+where
+  affine_env := sorry
+
+
 def isEnvsEntails (expr : Expr) : Bool := expr.isAppOfArity ``envs_entails 4
 
 def extractEnvsEntails? (expr : Expr) : Option (Expr × Expr × Expr) := Id.run <| do
