src/Iris/Std/List.lean
@@ -5,6 +5,12 @@ def isEmptyR : List α → Bool
   | []     => true
   | _ :: _ => false
 
+@[reducible]
+def eraseIdxR : List α → Nat → List α
+  | [], _          => []
+  | _ :: as, 0     => as
+  | a :: as, n + 1 => a :: eraseIdxR as n
+
 @[specialize]
 def foldl1 {α} (f : α → α → α) (alt : Unit → α) : List α → α
   | []     => alt ()
@@ -15,5 +21,10 @@ def foldr1 {α} (f : α → α → α) (alt : Unit → α) : List α → α
   | []     => alt ()
   | [a]    => a
   | a :: l => f a (foldr1 f alt l)
+
+@[reducible]
+def getR : (as : List α) → Fin as.length → α
+  | a::as, ⟨0, _⟩ => a
+  | a::as, ⟨Nat.succ i, h⟩ => getR as ⟨i, Nat.le_of_succ_le_succ h⟩
 
 end List
