src/Iris/Std.lean
@@ -1,5 +1,4 @@
 import Iris.Std.Classes
 import Iris.Std.Expr
 import Iris.Std.List
-import Iris.Std.Syntax
 import Iris.Std.TC
